Chapter2/Imp.lean
@@ -39,25 +39,6 @@ Updates the state by assigning a new value to a specified variable.
 def set (st: State) (x : String) (v: ℕ) : State :=
   fun y => if y = x then v else st y
 
-/--
-Syntax of commands in our simple imperative language.
-
-The inductive type `Command` represents the syntax with the following constructors:
-- `skip`: A no-operation command.
-- `assign`: Assigns a fixed natural number to a variable (`x := a`).
-- `assignvar`: Assigns the value of one variable to another (`x := y`).
-- `seq`: Sequential composition of two commands (`c1; c2`).
-- `if_`: Conditional command that executes one of two branches based on a boolean condition.
-- `while`: A while-loop that repeatedly executes a command as long as the condition is true.
--/
-inductive Command: Type
-| skip: Command                               -- nop
-| assign (x : String) (a: ℕ) : Command        -- x := a
-| assignvar (x: String) (y: String) : Command -- x := y
-| seq (c1 c2 : Command) : Command                 -- c1; c2
-| if_ (b : Bool) (c1 c2 : Command) : Command      -- if b then c1 else c2
-| while (b : Bool) (c : Command) : Command        -- while b do c
-
 -- inductive definitions in Lean come with an important implicit principle:
 -- ** the only ways to construct proofs of the inductive relation are through its constructors.
 
@@ -76,12 +57,12 @@ inductive AExp : Type
 | mul (a₁ a₂ : AExp) : AExp
 | sub (a₁ a₂ : AExp) : AExp
 
-def AEval : State → AExp → ℕ
-| _, .const n   => n
-| st, .var x     => st x
-| st, .add a₁ a₂ => AEval st a₁ + AEval st a₂
-| st, .mul a₁ a₂ => AEval st a₁ * AEval st a₂
-| st, .sub a₁ a₂ => AEval st a₁ - AEval st a₂
+inductive AEval : State → AExp → ℕ → Prop
+| const (st : State) (n : ℕ) : AEval st (.const n) n
+| var (st : State) (x : String) : AEval st (.var x) (get st x)
+| add (st : State) (a₁ a₂ : AExp) (n₁ n₂ : ℕ) : AEval st a₁ n₁ → AEval st a₂ n₂ → AEval st (.add a₁ a₂) (n₁ + n₂)
+| mul (st : State) (a₁ a₂ : AExp) (n₁ n₂ : ℕ) : AEval st a₁ n₁ → AEval st a₂ n₂ → AEval st (.mul a₁ a₂) (n₁ * n₂)
+| sub (st : State) (a₁ a₂ : AExp) (n₁ n₂ : ℕ) : AEval st a₁ n₁ → AEval st a₂ n₂ → AEval st (.sub a₁ a₂) (n₁ - n₂)
 
 inductive BExp : Type
 | btrue  : BExp
@@ -91,13 +72,32 @@ inductive BExp : Type
 | not (b : BExp) : BExp
 | and (b₁ b₂ : BExp) : BExp
 
-def BEval : State → BExp → Bool
-| _, .btrue       => true
-| _, .bfalse      => false
-| st, .eq a1 a2    => AEval st a1 = AEval st a2
-| st, .le a1 a2    => AEval st a1 ≤ AEval st a2
-| st, .not b       => ¬(BEval st b)
-| st, .and b1 b2   => (BEval st b1) && (BEval st b2)
+inductive BEval : State → BExp → Bool → Prop
+| btrue (st : State) : BEval st .btrue true
+| bfalse (st : State) : BEval st .bfalse false
+| eq (st : State) (a₁ a₂ : AExp) (n₁ n₂ : ℕ) : (AEval st a₁ n₁) → (AEval st a₂ n₂) → BEval st (.eq a₁ a₂) (n₁ = n₂)
+| le (st : State) (a₁ a₂ : AExp) (n₁ n₂ : ℕ) : (AEval st a₁ n₁) → (AEval st a₂ n₂) → BEval st (.eq a₁ a₂) (n₁ ≤ n₂)
+| not (st : State) (bexp : BExp) (b : Bool) : BEval st bexp b → BEval st (.not bexp) (¬b)
+| and (st : State) (bexp₁ bexp₂ : BExp) (b₁ b₂ : Bool) : (BEval st bexp₁ b₁) → (BEval st bexp₂ b₂) → BEval st (.and bexp₁ bexp₂) (b₁ && b₂)
+
+/--
+Syntax of commands in our simple imperative language.
+
+The inductive type `Command` represents the syntax with the following constructors:
+- `skip`: A no-operation command.
+- `assign`: Assigns a fixed natural number to a variable (`x := a`).
+- `assignvar`: Assigns the value of one variable to another (`x := y`).
+- `seq`: Sequential composition of two commands (`c1; c2`).
+- `if_`: Conditional command that executes one of two branches based on a boolean condition.
+- `while`: A while-loop that repeatedly executes a command as long as the condition is true.
+-/
+inductive Command: Type
+| skip: Command                               -- nop
+| assign (x : String) (a: AExp) : Command        -- x := a
+| seq (c1 c2 : Command) : Command                 -- c1; c2
+| if_ (b : BExp) (c1 c2 : Command) : Command      -- if b then c1 else c2
+| while (b : BExp) (c : Command) : Command        -- while b do c
+
 
 /--
 Inductive definition of command evaluation (`CEval`).
@@ -108,7 +108,6 @@ initial state `st` to a final state `st'` after executing a command.
 Constructors:
 - `skip`: Evaluating `skip` leaves the state unchanged.
 - `assign`: Evaluating an assignment updates the state with the new value for the variable.
-- `assignvar`: Evaluates an assignment where a variable is assigned the value of another variable.
 - `seq`: Sequentially composes two command evaluations.
 - `if_true`: Evaluates the "then" branch when the condition is true.
 - `if_false`: Evaluates the "else" branch when the condition is false.
@@ -118,19 +117,17 @@ Constructors:
 inductive CEval : Command -> State -> State -> Prop
 | skip (st : State) :
     CEval .skip st st
-| assign (st : State) (x : String) (n : ℕ) :
-    CEval (.assign x n) st (set st x n)
-| assignvar (st : State) (x : String) (y : String) :
-    CEval (.assignvar x y) st (set st x (get st y))
+| assign (st : State) (x : String) (a : AExp) (n : ℕ):
+    (AEval st a n) → CEval (.assign x a) st (set st x n)
 | seq (c1 c2 : Command) (st st' st'' : State) :
     CEval c1 st st' → CEval c2 st' st'' → CEval (.seq c1 c2) st st''
-| if_true (st st' : State) (c1 c2 : Command) :
-    CEval c1 st st' → CEval (.if_ true c1 c2) st st'
-| if_false (st st' : State) (b : Bool) (c1 c2 : Command) :
-    CEval c2 st st' → CEval (.if_ false c1 c2) st st'
-| while_false (st : State) (c : Command) :
-    CEval (.while false c) st st
-| while_true (st st' st'' : State) (c : Command) :
-    CEval c st st' → CEval (.while true c) st' st'' → CEval (.while true c) st st''
+| if_true (st st' : State) (b : BExp) (c1 c2 : Command) :
+    BEval st b true → CEval c1 st st' → CEval (.if_ b c1 c2) st st'
+| if_false (st st' : State) (b : BExp) (c1 c2 : Command) :
+    BEval st b false → CEval c2 st st' → CEval (.if_ b c1 c2) st st'
+| while_false (st : State) (b : BExp) (c : Command) :
+    BEval st b false → CEval (.while b c) st st
+| while_true (st st' st'' : State) (b : BExp) (c : Command) :
+    BEval st b true → CEval c st st' → CEval (.while b c) st' st'' → CEval (.while b c) st st''
 
 end Imp
